### Strukturelle Induktion

#### IB Induktionsbehauptung

Für alle beliebigen aber festen Listen `xs` gelte:

```haskell
sum (foo xs) = 2 * sum xs - length xs
```

#### IB Induktionsanfang

Zeige IB für `xs = []`:

```haskell
            sum (foo [])
{- (2) -} = sum []
{- (6) -} = 0
          = 2 * 0 - 0
{- (6) -} = 2 * sum [] - 0
{- (2) -} = 2 * sum [] - foo []
```

#### IV Induktionsvoraussetzung
```haskell
sum (foo xs) = 2 * sum xs - length xs
```

#### IS Induktionsschritt

Zeige IB für `xs = (x:xs')`:

```haskell
            sum (foo (x:xs'))
{- (3) -} = sum (x : x : (-1) : foo (xs'))
{- (7) -} = x + sum (x : (-1) : foo (xs'))
{- (7) -} = x + x + sum ((-1) : foo (xs'))
{- (7) -} = x + x + (-1) + sum (foo (xs'))
{- IV  -} = x + x + (-1) + 2 * sum xs' - length xs'
          = 2  * (x + sum xs') - (1 + length xs')
{- (7) -} = 2 * sum (x:xs') - (1 + length xs')
{-(11) -} = 2 * sum (x:xs') - length (x:xs')
```

