\documentclass[t]{beamer}
%NewComand definitions
\usepackage{xparse}
\usepackage{fontspec}
\usepackage{amsmath}
\usepackage{mathtools}
\usepackage{unicode-math}
\usepackage{listings}

\NewDocumentCommand\FV{}{\alert<2>}
\NewDocumentCommand\GV{}{\alert<3>}
\NewDocumentCommand\alphaconversion{}{\Rightarrow_α}
\NewDocumentCommand\betareduction{}{\Rightarrow_β}

\begin{document}

\begin{frame}{Aufgabe 02a}

  \begin{gather*}
    (λfx.\underbrace{fx}_{GV = \{f, x\}} )(\underbrace{λzy.xy}_{FV=\{x\}})x \\
    \uncover<2->{
      \alphaconversion (λfx'. \underbrace{fx'}_{GV=\{f,x'\}})(\underbrace{λzy.xy}_{FV=\{x\}})x \\    
    }
    \uncover<3->{
      \betareduction (λx'. \underbrace{(λzy.xy)x'}_{GV=\{x'\}}) \underbrace{x}_{FV=\{x\}} \\
    }
    \uncover<4->{
      \betareduction (λzx.\underbrace{xy}_{GV=\{y\}}) \underbrace{x}_{FV=\{x\}} \\
    }
    \uncover<5->{
      \betareduction (λy.xy)
    }
  \end{gather*}
\end{frame}

\begin{frame}{Aufgabe 2b}
  \frametitle{Aufgabe 2b}
  \lstinputlisting[language=Haskell]{A2b.hs}
$\langle G\rangle =  ( ( λgxy.\langle ite\rangle  (\langle iszero\rangle  y)$ \\
$        ( \langle ite\rangle  (\langle iszero\rangle  (\langle pred\rangle  y))$ \\
$          ( g (\langle succ\rangle  x)          (\langle pred\rangle  y))$ \\
$          ( g (\langle succ\rangle  (\langle succ\rangle  x)) (\langle pred\rangle  (\langle pred\rangle  y)))$ \\
$        )    $
$      ) $
\end{frame}
\end{document}