3a
```
(λxyz.yzx)(λx.xy)(λx.x)
GV(λyz.yzx)={y,z}, FV(λx.xy)={y}
=>α
(λxyz.y'zx)(λx.xy)(λx.x)
GV(λy'z.y'zx)={y',z}, FV(λx.xy)={y}
=>β
(λy'z.y'z(λx.xy))(λx.x)
GV(λz.y'z(λx.xy))={z,x},FV(λx.x)={}
=>β
(λz.(λx.x)z(λx.xy))
GV(x)={}, FV(z)={z}
=>β
(λz.z(λx.xy))
```

3b
```Haskell
g :: Int -> Int -> Int -> Int
g 0 _ _ = 0
g n x y = (g (n - 1) x y) + (if n ‘mod‘ 2 == 0 then x else y)
```
In λ-Term
```
<G> =
(λgnxy.<ite> (<iszero> x)
  <0>
  (<add>
   (g (<pred> n) x y)
   (<ite> (<iszero> (<mod> n <2>)) x y)
  )
)
```

3c
```
<F> = 
(λfnxy.<ite>(<iszero> (<pred> n))
  (<add> x y)
  (f (<pred> n) (<mult> x n) (<add> y n))
)
```

Zuerst löst man die Abstraktion über dem Fixpunktkombinator auf
```
<Y> <F>  = (λh.((λy.h(yy))(λy.h(yy)))) <F>
=>β 
(λy.<F> (yy)) (λy.<F> (yy)) = t_F t_F
=>β
<Y>  (λy.<F> (yy))(λy.<F> (yy)) = <F>  (t_F t_F)
```

Nun kann man weiter den Term vereinfachen.
```
<F>(t_F t_F) <2><3><5>= 
(λfnxy.<ite>(<iszero> (<pred> n))
  (<add> x y)
  (f (<pred> n) (<mult> x n) (<add> y n))
)(t_F t_F) <2><3><5>
=>*β
(<ite>(<iszero> (<pred> <2>))
  (<add> <3> <5>)
  ((t_F t_F) (<pred> <2>) (<mult> <3> <2>) (<add> <5> <2>))
) 
=>*β
(<ite>(<false>)
  (<add> <3> <5>)
  (<F> (t_F t_F) <1> <6> <7>)
) 
=>*β
<F> (t_F t_F) <1> <6> <7> =
(λfnxy.<ite>(<iszero> (<pred> n))
  (<add> x y)
  (f (<pred> n) (<mult> x n) (<add> y n))
)(t_F t_F) <1><6><7>
=>*β
(<ite>(<iszero> (<pred> <1>))
  (<add> <6> <7>)
  ((t_F t_F) (<pred> <1>) (<mult> <6> <1>) (<add> <7> <1>))
) 
=>*β
(<ite> (<true>)
  <13>
  ((t_F t_F) (<pred> <1>) (<mult> <6> <1>) (<add> <7> <1>))
) 
=>*β
<13>
```