\documentclass[t]{beamer}
\usepackage{xparse}
\usepackage{fontspec}
\usepackage{amsmath}
\usepackage{mathtools}
\usepackage{unicode-math}

\NewDocumentCommand\FV{}{\alert<2>}
\NewDocumentCommand\GV{}{\alert<3>}
\NewDocumentCommand\alphaconversion{}{\Rightarrow_α}
\NewDocumentCommand\betareduction{}{\Rightarrow_β}

\begin{document}

\begin{frame}{Aufgabe 4a}
  \begin{gather*}
    (λ \GV{x} . x  \FV{y}) (λ \GV{y}.y) \\
    \uncover<2->{
      FV = \{ y \} \\
    }
    \uncover<3->{
      GV = \{ x, y \}
    }
  \end{gather*}
\end{frame}

\begin{frame}{Aufgabe 4a}
  \begin{gather*}
    (λ \GV{x} . (λ \GV{y} . \FV{z} (λ \GV{z} . z (λ \GV{x} . y)))) \\
    \uncover<2->{
      FV = \{ z \} \\
    }
    \uncover<3->{
      GV = \{ x, y, z \}
    }
  \end{gather*}
\end{frame}

\begin{frame}{Aufgabe 4a}
  \begin{gather*}
    (λ \GV{x} . (λ \GV{y} . x \FV{z} ( y \FV{z} ))) (λ \GV{x} . \FV{y} (λ \GV{y} . y )) \\
    \uncover<2->{
      FV = \{ y, z \} \\
    }
    \uncover<3->{
      GV = \{ x, y \}
    }
  \end{gather*}
\end{frame}


\begin{frame}{Aufgabe 4b}
  \begin{align*}
    \uncover<+->{
      &
      (λ x . \underbrace{(λ y . x z ( y z ))}_{GV = \{ y \}}) \underbrace{(λ x . y (λ y . y ))}_{FV = \{ y \}}
      \\
    }
    \uncover<+->{
      \alphaconversion
      &
      (λ x . (λ y' . x z ( y' z ))) (λ x . y (λ y . y ))
      \\
    }
    \uncover<+->{
      \betareduction
      &
      (λ y' . (λ x . \underbrace{y (λ y . y )}_{GV = \{y\}}) \underbrace{\vphantom{(}z}_{FV = \{z\}} ( y' z ))
      \\
    }
    \uncover<+->{
      \betareduction
      &
      (λ y' . y (λ y . y ) ( y' z ))
      \\
    }
  \end{align*}
\end{frame}

\begin{frame}{Aufgabe 4b (restliche Lösungen)}
  \begin{equation*}
    (λx.(λ y.(λz.z))) x (+ y 1) \Rightarrow^{*} (λz.z)
  \end{equation*}

  \begin{equation*}
    (λx.(λ y.x (λz. y z))) (((λx.(λ y. y)) 8) (λx.(λ y. y) x)) \Rightarrow^{*} (λ y z. y z)
  \end{equation*}

  \begin{align*}
          & (λh.(λx.h (x x)) (λx.h (x x))) ((λx.x) (+ 1 5)) \\
    {}\Rightarrow^{*}{} & (λx. (+ 1 5) (x x)) (λx. (+ 1 5) (x x)) \\
    {}\Rightarrow^{*}{} & (λx. (+ 1 5) ((λx. (+ 1 5) (x x)) (λx. (+ 1 5) (x x)))) \\
    {}\Rightarrow^{*}{} & … \quad \text{(endlose Rekursion)}
  \end{align*}

  \begin{equation*}
    (λ f .(λa.(λb. f a b))) (λx.(λ y.x)) \Rightarrow^{*} (λa.(λb.a))
  \end{equation*}
\end{frame}

\end{document}
