2a)
```
(λxy.y(λx.x))(y(λx.x))z
GV(λy.y(λx.x))={x,y}, FV(y(λx.x))={y}
=>α
(λxy'.y'(λx.x))(y(λx.x))z
GV(λy'.y'(λx.x))={x,y'}, FV(y(λx.x))={y}
=>β
(λy'.y'(λx.x))z
GV(y'(λx.x))={x,y'}, FV(z)={z}
=>β
z(λx.x)
```

2b
```
<G> = 
(λgxy.
<ite>(<iszero>x)
  y
  (<ite>(<iszero>(<pred>x))
    (<mult><2>y)
    (<mult>
      (g (<pred>x)y)
      (g (<pred>(<pred>x)) (<succ> y))
    )
  )
)
```

```Haskell
-- <Y><G>
g :: Int -> Int -> Int
g 0 y = y
g 1 y = 2*y
g x y = (g (x-1) y) * (g (x-2) (y+1))
```

2c
```
<F> = 
(λfxyz.
<ite>(<iszero>y)
  (<add>xx)
  (<mult>
    z
    (f (<succ>x) (<pred>y) z)
  )
)
```
Zuerst löst man die Abstraktion über dem Fixpunktkombinator auf
```
<Y> <F>  = (λh.((λy.h(yy))(λy.h(yy)))) <F>
=>β 
(λy.<F> (yy)) (λy.<F> (yy)) = t_F t_F
=>β
<Y>  (λy.<F> (yy))(λy.<F> (yy)) = <F>  (t_F t_F)
```
Nun kann man weiter den Term vereinfachen.
```
<F>(t_F t_F)<4><1><2>=
(λfxyz.
<ite>(<iszero>y)
  (<add>xx)
  (<mult>
    z
    (f (<succ>x) (<pred>y) z)
  )
)(t_F t_F)<4><1><2>
=>*β
<ite>(<iszero><1>)
  (<add><4><4>)
  (<mult>
    <2>
    ((t_F t_F) (<succ><4>) (<pred><1>) <2>)
  )
=>*β
(<mult>
  <2>
  ((t_F t_F) <5> <0> <2>)
)
=>*β
(<mult>
  <2>
  (<F>(t_F t_F) <5> <0> <2>)
)
=>*β
(<mult>
  <2>
  (<ite>(<iszero><0>)
    (<add><5><5>)
    (<mult>
      <2>
      ((t_F t_F) (<succ><5>) (<pred><0>) <2>)
  )
)
=>*β
(<mult>
  <2>
  <10>
)
=>*β
<20>
```